src/ursus/CUE/Props.v
@@ -15,8 +15,6 @@ Require Import UMLang.GlobalClassGenerator.ClassGenerator.
 Require Import UrsusStdLib.Solidity.All.
 Require Import UrsusStdLib.Solidity.unitsNotations.
 Require Import UrsusTVM.Solidity.All.
-Require Export UrsusContractCreator.UrsusDefinitions.
-Require Export UrsusContractCreator.ReverseTranslatorConstructions.
 
 Import UrsusNotations.
 Local Open Scope xlist_scope.
@@ -47,7 +45,7 @@ Definition dummyRequest : UpdateRequestLRecord := Eval compute in default.
 
 Definition REU_1 l id (codeHash :  option uint256) (owners :  optional (listArray uint256)) (reqConfirms : optional uint8) (lifetime :  optional   uint32) : Prop := 
   let m_lifetime := uint2N (toValue (eval_state (sRReader (m_lifetime_right rec def) ) l)) in (* TODO *)
-  let tvm_now := uint2N (toValue (eval_state (sRReader || now ) l)) in
+  let tvm_now := uint2N (toValue (eval_state (sRReader || now ||) l)) in
   let l' := exec_state (Uinterpreter (_removeExpiredTransactions rec def)) l in 
   let ret_l := exec_state (Uinterpreter (_removeExpiredUpdateRequests rec def)) l in 
   let m_updateRequests := toValue (eval_state (sRReader (m_updateRequests_right rec def) ) l) in
@@ -62,14 +60,14 @@ Definition REU_1 l id (codeHash :  option uint256) (owners :  optional (listArra
 
 
 Definition CUE_1 l (updateId :  uint64) (code : optional cell_) : Prop :=
-  let msgPubkey := toValue (eval_state (sRReader || msg->pubkey()  ) l) in
+  let msgPubkey := toValue (eval_state (sRReader || msg->pubkey() || ) l) in
   let custodians := toValue (eval_state (sRReader (m_custodians_right rec def) ) l) in
   isError (eval_state (Uinterpreter (executeUpdate rec def updateId code)) l) = false -> 
   hmapIsMember msgPubkey custodians = true.
 
 Definition CUE_2 l id (updateId :  uint64) (code : optional cell_) (custodianIndex :  uint8) (codeHash : optional uint256) (owners : optional (listArray uint256)) (reqConfirms : optional uint8) (lifetime :  optional   uint32) : Prop := 
   let custodians := toValue (eval_state (sRReader (m_custodians_right rec def) ) l) in
-  let msgPubkey := toValue (eval_state (sRReader || msg->pubkey() ) l) in
+  let msgPubkey := toValue (eval_state (sRReader || msg->pubkey() ||) l) in
   let l' := exec_state (Uinterpreter (_confirmUpdate rec def updateId custodianIndex)) l in
   let transactions := toValue (eval_state (sRReader (m_transactions_right rec def) ) l') in
   correctState l ->
@@ -109,7 +107,7 @@ Definition CUE_6_2 l (updateId :  uint64)  (code : optional cell_) : Prop :=
   let m_updateRequests_old := toValue (eval_state (sRReader (m_updateRequests_right rec def) ) l) in
   let m_lifetime := toValue (eval_state (sRReader (m_lifetime_right rec def) ) l') in
   let m_lifetime_old := toValue (eval_state (sRReader (m_lifetime_right rec def) ) l) in
-  let tvm_now := uint2N (toValue (eval_state (sRReader || now ) l)) in
+  let tvm_now := uint2N (toValue (eval_state (sRReader || now ||) l)) in
   let expiredRequests := xHMapFilter (fun k v =>
     N.leb ((N.shiftr (uint2N k) 32) + uint2N m_lifetime_old) tvm_now
   ) m_updateRequests_old in
@@ -120,10 +118,10 @@ Definition CUE_6_2 l (updateId :  uint64)  (code : optional cell_) : Prop :=
   let owners := getPruvendoRecord UpdateRequest_ι_custodians ur in 
   let reqConfirms := getPruvendoRecord UpdateRequest_ι_reqConfirms ur in 
   let lifetime := getPruvendoRecord UpdateRequest_ι_lifetime ur in
-  let ecode := (toValue (eval_state (sRReader || tvm->code() ) l')) in
-  let ecode_old := (toValue (eval_state (sRReader || tvm->code() ) l)) in
-  let ccode := (toValue (eval_state (sRReader || tvm->currentCode() ) l')) in
-  let ccode_old := (toValue (eval_state (sRReader || tvm->currentCode() ) l)) in
+  let ecode := (toValue (eval_state (sRReader || tvm->code() ||) l')) in
+  let ecode_old := (toValue (eval_state (sRReader || tvm->code() ||) l)) in
+  let ccode := (toValue (eval_state (sRReader || tvm->currentCode() ||) l')) in
+  let ccode_old := (toValue (eval_state (sRReader || tvm->currentCode() ||) l)) in
   let m_custodians := toValue (eval_state (sRReader (m_custodians_right rec def) ) l') in
   let m_custodians_old := toValue (eval_state (sRReader (m_custodians_right rec def) ) l) in
   let m_ownerKey_old := toValue (eval_state (sRReader (m_ownerKey_right rec def) ) l) in
