src/ursus/MTS/Props.v
@@ -15,8 +15,6 @@ Require Import UMLang.GlobalClassGenerator.ClassGenerator.
 Require Import UrsusStdLib.Solidity.All.
 Require Import UrsusStdLib.Solidity.unitsNotations.
 Require Import UrsusTVM.Solidity.All.
-Require Export UrsusContractCreator.UrsusDefinitions.
-Require Export UrsusContractCreator.ReverseTranslatorConstructions.
 
 Import UrsusNotations.
 Local Open Scope xlist_scope.
@@ -50,7 +48,7 @@ Definition ETR_1 l u (dest :  address) (value :  uint128) (bounce :  boolean) (a
   let lifetime := uint2N (toValue (eval_state (sRReader (m_lifetime_right rec def) ) l)) in
   let MAX_CLEANUP_TXNS := uint2N (toValue (eval_state (sRReader (MAX_CLEANUP_TXNS_right rec def) ) l)) in
   let m_updateRequests := toValue (eval_state (sRReader (m_updateRequests_right rec def) ) l) in
-  let tvm_now := uint2N (toValue (eval_state (sRReader || now ) l)) in
+  let tvm_now := uint2N (toValue (eval_state (sRReader || now ||) l)) in
   let id := (getPruvendoRecord Transaction_ι_id u) in
   let l' := exec_state (Uinterpreter (_removeExpiredTransactions rec def)) l in 
   let m_transactions := toValue (eval_state (sRReader (m_transactions_right rec def) ) l') in
@@ -64,14 +62,14 @@ Definition ETR_1 l u (dest :  address) (value :  uint128) (bounce :  boolean) (a
 
 Definition MTS_1 l (dest :  address) (value :  uint128) (bounce :  boolean) (allBalance :  boolean) (payload :  cell_) (stateInit :  optional  ( TvmCell )) : Prop := 
   let custodians := toValue (eval_state (sRReader (m_custodians_right rec def) ) l) in
-  let msgPubkey := toValue (eval_state (sRReader || msg->pubkey() ) l) in
+  let msgPubkey := toValue (eval_state (sRReader || msg->pubkey() ||) l) in
   correctState l ->
   isError (eval_state (Uinterpreter (submitTransaction rec def dest value bounce allBalance payload stateInit)) l) = false ->
   hmapIsMember msgPubkey custodians = true.
 
 Definition MTS_2 l id (dest :  address) (value :  uint128) (bounce :  boolean) (allBalance :  boolean) (payload :  cell_) (stateInit :  optional  ( TvmCell )) : Prop := 
   let custodians := toValue (eval_state (sRReader (m_custodians_right rec def) ) l) in
-  let msgPubkey := toValue (eval_state (sRReader || msg->pubkey() ) l) in
+  let msgPubkey := toValue (eval_state (sRReader || msg->pubkey() ||) l) in
   let l' := exec_state (Uinterpreter (submitTransaction rec def dest value bounce allBalance payload stateInit)) l in 
   let transactions := toValue (eval_state (sRReader (m_transactions_right rec def) ) l') in
   let u := xMaybeMapDefault (fun x => x) (hmapLookup id transactions) dummyTransaction  in  
@@ -84,13 +82,13 @@ Definition MTS_2 l id (dest :  address) (value :  uint128) (bounce :  boolean) (
 Definition MTS_3 l (dest :  address) (value :  uint128) (bounce :  boolean) (allBalance :  boolean) (payload :  cell_) (stateInit :  optional  ( TvmCell )) : Prop := 
   let custodians := toValue (eval_state (sRReader (m_custodians_right rec def) ) l) in
   let requestsMask := toValue (eval_state (sRReader (m_requestsMask_right rec def) ) l) in 
-  let msgPubkey := toValue (eval_state (sRReader || msg->pubkey() ) l) in
+  let msgPubkey := toValue (eval_state (sRReader || msg->pubkey() ||) l) in
   let i := uint2N (hmapFindWithDefault (Build_XUBInteger 0) msgPubkey custodians) in
   let bitsMask := N.land (N.shiftr (uint2N requestsMask) (8 * i)) 255 in
   let transactions := toValue (eval_state (sRReader (m_transactions_right rec def) ) l) in
   let lifetime := uint2N (toValue (eval_state (sRReader (m_lifetime_right rec def) ) l)) in
   let MAX_QUEUED_REQUESTS := uint2N (toValue (eval_state (sRReader (MAX_QUEUED_REQUESTS_right rec def) ) l)) in
-  let tvm_now := uint2N (toValue (eval_state (sRReader || now ) l)) in
+  let tvm_now := uint2N (toValue (eval_state (sRReader || now ||) l)) in
   let expiredTransactions := xHMapFilter (fun k v =>
     let index := uint2N (getPruvendoRecord Transaction_ι_index v) in
     andb (N.eqb index i) (N.leb ((N.shiftr (uint2N k) 32) + lifetime) tvm_now)
@@ -106,7 +104,7 @@ Definition MTS_4 l id (dest :  address) (value :  uint128) (bounce :  boolean) (
   let custodians := toValue (eval_state (sRReader (m_custodians_right rec def) ) l) in
   let requestsMask :=  (toValue (eval_state (sRReader (m_requestsMask_right rec def) ) l)) in
   let m_defaultRequiredConfirmations :=  uint2N (toValue (eval_state (sRReader (m_defaultRequiredConfirmations_right rec def) ) l)) in (* ???? *)
-  let msgPubkey := toValue (eval_state (sRReader || msg->pubkey() ) l) in
+  let msgPubkey := toValue (eval_state (sRReader || msg->pubkey() ||) l) in
   let l' := exec_state (Uinterpreter (submitTransaction rec def dest value bounce allBalance payload stateInit)) l in
   let messqueue := toValue ((eval_state (sRReader (ULtoRValue (IDefault_left rec def)))) l') in 
   let mes := EmptyMessage IDefault (Build_XUBInteger 0, (bounce, (Build_XUBInteger (N.lor FLAG_IGNORE_ERRORS FLAG_SEND_ALL_REMAINING) , payload))) in
@@ -116,7 +114,7 @@ Definition MTS_4 l id (dest :  address) (value :  uint128) (bounce :  boolean) (
   let bitsMask := N.land (N.shiftr (uint2N requestsMask) (8 * i)) 255 in
   let lifetime := uint2N (toValue (eval_state (sRReader (m_lifetime_right rec def) ) l)) in
   let MAX_QUEUED_REQUESTS := uint2N (toValue (eval_state (sRReader (MAX_QUEUED_REQUESTS_right rec def) ) l)) in
-  let tvm_now := uint2N (toValue (eval_state (sRReader || now ) l)) in
+  let tvm_now := uint2N (toValue (eval_state (sRReader || now ||) l)) in
   let expiredTransactions := xHMapFilter (fun k v =>
     let index := uint2N (getPruvendoRecord Transaction_ι_index v) in
     andb (N.eqb index i) (N.leb ((N.shiftr (uint2N k) 32) + lifetime) tvm_now)
@@ -139,7 +137,7 @@ Definition MTS_5 l id (dest :  address) (value :  uint128) (bounce :  boolean) (
   let custodians := toValue (eval_state (sRReader (m_custodians_right rec def) ) l) in
   let requestsMask := (toValue (eval_state (sRReader (m_requestsMask_right rec def) ) l)) in
   let m_defaultRequiredConfirmations :=  uint2N (toValue (eval_state (sRReader (m_defaultRequiredConfirmations_right rec def) ) l)) in (* ???? *)
-  let msgPubkey := toValue (eval_state (sRReader || msg->pubkey() ) l) in
+  let msgPubkey := toValue (eval_state (sRReader || msg->pubkey() ||) l) in
   let l' := exec_state (Uinterpreter (submitTransaction rec def dest value bounce allBalance payload stateInit)) l in
   let messqueue := toValue ((eval_state (sRReader (ULtoRValue (IDefault_left rec def)))) l') in 
   let mes := EmptyMessage IDefault (value, (bounce, ((Build_XUBInteger  (N.lor FLAG_IGNORE_ERRORS FLAG_PAY_FWD_FEE_FROM_BALANCE)), payload))) in
@@ -149,7 +147,7 @@ Definition MTS_5 l id (dest :  address) (value :  uint128) (bounce :  boolean) (
   let bitsMask := N.land (N.shiftr (uint2N requestsMask) (8 * i)) 255 in
   let lifetime := uint2N (toValue (eval_state (sRReader (m_lifetime_right rec def) ) l)) in
   let MAX_QUEUED_REQUESTS := uint2N (toValue (eval_state (sRReader (MAX_QUEUED_REQUESTS_right rec def) ) l)) in
-  let tvm_now := uint2N (toValue (eval_state (sRReader || now ) l)) in
+  let tvm_now := uint2N (toValue (eval_state (sRReader || now ||) l)) in
   let expiredTransactions := xHMapFilter (fun k v =>
     let index := uint2N (getPruvendoRecord Transaction_ι_index v) in
     andb (N.eqb index i) (N.leb ((N.shiftr (uint2N k) 32) + lifetime) tvm_now)
@@ -188,13 +186,13 @@ Definition MTS_6_3  l (dest :  address) (value :  uint128) (bounce :  boolean) (
   let IGNORE_ERRORS := uint2N (toValue (eval_state (sRReader (FLAG_IGNORE_ERRORS_right rec def) ) l)) in
   let SEND_ALL_REMAINING := uint2N (toValue (eval_state (sRReader (FLAG_SEND_ALL_REMAINING_right rec def) ) l)) in
   let PAY_FWD_FEE_FROM_BALANCE := uint2N (toValue (eval_state (sRReader (FLAG_PAY_FWD_FEE_FROM_BALANCE_right rec def) ) l)) in
-  let msgPubkey := toValue (eval_state (sRReader || msg->pubkey() ) l) in
+  let msgPubkey := toValue (eval_state (sRReader || msg->pubkey() ||) l) in
   let i := uint2N (hmapFindWithDefault (Build_XUBInteger 0) msgPubkey custodians) in
   let m_defaultRequiredConfirmations := uint2N (toValue (eval_state (sRReader (m_defaultRequiredConfirmations_right rec def) ) l)) in
   let requestsMask := toValue (eval_state (sRReader (m_requestsMask_right rec def) ) l) in 
   let bitsMask := N.land (N.shiftr (uint2N requestsMask) (8 * i)) 255 in
   let lifetime := uint2N (toValue (eval_state (sRReader (m_lifetime_right rec def) ) l)) in
-  let tvm_now := uint2N (toValue (eval_state (sRReader || now ) l)) in
+  let tvm_now := uint2N (toValue (eval_state (sRReader || now ||) l)) in
   let expiredTransactions := xHMapFilter (fun k v =>
     let index := uint2N (getPruvendoRecord Transaction_ι_index v) in
     andb (N.eqb index i) (N.leb ((N.shiftr (uint2N k) 32) + lifetime) tvm_now)
@@ -223,7 +221,7 @@ Definition MTS_6_3  l (dest :  address) (value :  uint128) (bounce :  boolean) (
 Definition equalExceptLocalExpired (l l': LedgerLRecord rec) := 
   let transactions := toValue (eval_state (sRReader (m_transactions_right rec def) ) l) in
   let lifetime := uint2N (toValue (eval_state (sRReader (m_lifetime_right rec def) ) l)) in
-  let tvm_now := uint2N (toValue (eval_state (sRReader || now ) l)) in
+  let tvm_now := uint2N (toValue (eval_state (sRReader || now ||) l)) in
   let newTransactions : field_type _m_transactions := xHMapFilter (fun k v =>
     negb (N.leb ((N.shiftr (uint2N k) 32) + lifetime) tvm_now)
   ) transactions in
@@ -244,7 +242,7 @@ Definition equalExceptLocal (l l': LedgerLRecord rec) :=
 Definition MTS_7 l (dest :  address) (value :  uint128) (bounce :  boolean) (allBalance :  boolean) (payload :  cell_) (stateInit :  optional  ( TvmCell )) : Prop := 
   let l' := exec_state (Uinterpreter (submitTransaction rec def dest value bounce allBalance payload stateInit)) l in 
   let lifetime := uint2N (toValue (eval_state (sRReader (m_lifetime_right rec def) ) l)) in
-  let tvm_now := uint2N (toValue (eval_state (sRReader || now ) l)) in
+  let tvm_now := uint2N (toValue (eval_state (sRReader || now ||) l)) in
   correctState l ->
   isError (eval_state (Uinterpreter (submitTransaction rec def dest value bounce allBalance payload stateInit)) l) = true ->
   equalExceptLocalExpired l l' = true \/
